proof/refine/ARM/ADT_H.thy
@@ -319,6 +319,9 @@ fun
 | "CapabilityMap (capability.ArchObjectCap
                     (arch_capability.PageDirectoryCap word data)) =
   cap.ArchObjectCap (arch_cap.PageDirectoryCap word data)"
+| "CapabilityMap (capability.ArchObjectCap
+                    (arch_capability.SGISignalCap irq target)) =
+  cap.ArchObjectCap (arch_cap.SGISignalCap (ucast irq) (ucast target))"
 
 (* FIXME: wellformed_cap_simps has lots of duplicates. *)
 lemma cap_relation_imp_CapabilityMap:
@@ -335,7 +338,7 @@ lemma cap_relation_imp_CapabilityMap:
    apply (simp add: zbits_map_def split: option.splits)
   apply (rename_tac arch_cap)
   apply clarsimp
-  apply (case_tac arch_cap, simp_all add: wellformed_cap_simps)
+  apply (case_tac arch_cap, simp_all add: wellformed_cap_simps ucast_ucast_id)
   done
 
 primrec
